Lemmas about strings... but unfortunately I proved things about prefixes, not suffixes. Oops.

parser/Parser.fst
@@ -10,39 +10,27 @@ or the parse_error type.
 
 open FStar.String
 open FStar.Printf
+open FStar.Tactics
+open StringLemmas
 
 // The type returned by a parser
 type parse_result 'a =
   | ParseError : expecting:string -> at:string -> parse_result 'a
   | Success : v:'a -> rest:string -> parse_result 'a
 
-// Need to define substrings to state that the parser consumes
-// a portion of the input and leaves the rest.
-let is_proper_substring (a:string) (b:string) : bool = 
-  if strlen a = 0 then false else
-  if strlen a > strlen b then false else
-  (sub b 0 (strlen a)) = a
-
-let proper_substring_is_shorter (a:string) (b:string) 
-  : Lemma (requires (is_proper_substring a b))
-          (ensures (strlen a) < (strlen b) )
-           = admit()
-        
-// Lemma: a substring of a substring is a substring
-let substring_transitivity (a:string) (b:string) (c:string) :
-  Lemma (requires (is_proper_substring a b) && (is_proper_substring b c))
-        (ensures (is_proper_substring a c)) 
-          = admit()
-
 // The type of a parser 
-type parser 'a = (x:string) -> Tot (parse_result 'a)
+type parser 'a = (x:string) -> Tot (r:(parse_result 'a){ParseError? r ||
+  is_substring (Success?.rest r) x})
 
-// A parser that is guaranteed to consume at least one unit
-type proper_parser 'a = (x:string) -> Tot (r:(parse_result 'a){ParseError? r ||
-  is_proper_substring (Success?.rest r) x})
+// Transform the result of a single parser
+let parse_apply #a #b (f:a->b) (x:(parser a)) : (parser b) =
+  fun (input:string) -> 
+  match (x input) with
+  | ParseError e1 a1 -> ParseError e1 a1
+  | Success t1 rest -> Success (f t1) rest
 
 // Parse one type, then a second, and return a pair
-let parse_seq #a #b (x:(proper_parser a)) (y:(proper_parser b)) : Tot (proper_parser (a*b)) =
+let parse_seq #a #b (x:(parser a)) (y:(parser b)) : Tot (parser (a*b)) =
   fun (input:string) -> 
   match (x input) with
   | ParseError e1 a1 -> ParseError e1 a1
@@ -54,11 +42,11 @@ let parse_seq #a #b (x:(proper_parser a)) (y:(proper_parser b)) : Tot (proper_pa
           Success (t1, t2) r2 )
 
 //  <,> to create pairs
-let op_Less_Comma_Greater (#a:Type) (#b:Type) (x:proper_parser a) (y:proper_parser b) = 
+let op_Less_Comma_Greater (#a:Type) (#b:Type) (x:parser a) (y:parser b) = 
   parse_seq #a #b x y
 
 // Parse a list of one type, then a second list of the same type, and append them
-let parse_list #a (x:(proper_parser (list a))) (y:(proper_parser (list a))) : Tot (proper_parser (list a)) =
+let parse_list #a (x:(parser (list a))) (y:(parser (list a))) : Tot (parser (list a)) =
   fun (input:string) -> 
   match (x input) with
   | ParseError e1 a1 -> ParseError e1 a1
@@ -68,12 +56,24 @@ let parse_list #a (x:(proper_parser (list a))) (y:(proper_parser (list a))) : To
         (substring_transitivity r2 rest input;
          Success (FStar.List.Tot.append t1 t2) r2)
 
+// TODO: how to combine this with the above?
+let parse_nonempty_list #a (x:(parser (z:(list a){Cons? z}))) (y:(parser (list a))) 
+ : Tot (parser (z:(list a){Cons? z})) =
+  fun (input:string) -> 
+  match (x input) with
+  | ParseError e1 a1 -> ParseError e1 a1
+  | Success t1 rest -> match (y rest) with
+      | ParseError e2 a2 -> ParseError e2 a2 
+      | Success t2 r2 -> 
+        (substring_transitivity r2 rest input;
+         Success (FStar.List.Tot.append t1 t2) r2)
+ 
 // <::> to create lists
-let op_Less_Colon_Colon_Greater (#a:Type) (x:proper_parser (list a)) (y:proper_parser (list a)) =
+let op_Less_Colon_Colon_Greater (#a:Type) (x:parser (list a)) (y:parser (list a)) =
   parse_list #a x y
 
 // Explicitly combine the parse results from two types into a third
-let parse_comb #a #b #c (x:(proper_parser a)) (f: a -> b -> Tot c) (y:(proper_parser b)) : Tot (proper_parser (c)) =
+let parse_comb #a #b #c (x:(parser a)) (f: a -> b -> Tot c) (y:(parser b)) : Tot (parser (c)) =
   fun (input:string) -> 
   match (x input) with
   | ParseError e1 a1 -> ParseError e1 a1
@@ -101,7 +101,7 @@ let or_of_reasons #a (r1:string) (r2:string) (at:string)
     
 // Parse one of two options of the same type. Does not indicate which was chosen,
 // you'll have to have the value indicate that.
-let parse_either #a #b (x:(parser a)) (y:(parser a)) : Tot (parser a) =
+let parse_either #a (x:(parser a)) (y:(parser a)) : Tot (parser a) =
   fun (input:string) -> 
   match (x input) with
   | Success t1 rest -> Success t1 rest
@@ -109,13 +109,17 @@ let parse_either #a #b (x:(parser a)) (y:(parser a)) : Tot (parser a) =
      | Success t2 r2 -> Success t2 r2 
      | ParseError e2 a2 -> or_of_reasons e1 e2 input
 
+// <|> to create alternatives
+let op_Less_Bar_Greater (#a:Type) (x:(parser a)) (y:(parser a)) =
+  parse_either x y
+
 type left_right 'a 'b =
  | Left : left:'a -> left_right 'a 'b
  | Right :  right:'b -> left_right 'a 'b
  
 // Parse one of the options of differing types.  Indicate which was chosen with the
 // left_right type.
-let parse_lr #a #b (x:(proper_parser a)) (y:(proper_parser b)) : Tot (proper_parser (left_right a b)) =
+let parse_lr #a #b (x:(parser a)) (y:(parser b)) : Tot (parser (left_right a b)) =
   fun (input:string) -> 
   match (x input) with
   | Success t1 rest -> Success (Left t1) rest
@@ -123,28 +127,48 @@ let parse_lr #a #b (x:(proper_parser a)) (y:(proper_parser b)) : Tot (proper_par
      | Success t2 r2 -> Success (Right t2) r2 
      | ParseError e2 a2 -> or_of_reasons e1 e2 input
 
-// We can only parse a Kleene star if the parser guarantees it consumes at least one
-// token of the input each time.
-let rec parse_star_aux #a (input:string) (x:proper_parser a) (prev_a:list a) 
-: Tot (list a*string) (decreases (strlen input)) =
+// The Kleene star won't terminate if the parser doesn't consume input.  So, we'll
+// enforce totality by exiting as soon as it doesn't. 
+// (Previous approach: define proper and improper parsers, but then we'd have to have
+// make multiple version of the above combinators, probably?)
+let rec parse_star_aux #a (input:string) (x:parser a) (prev_a:list a) 
+: Tot ((list a)*(remaining:string{is_substring remaining input})) 
+  (decreases (strlen input)) =
   match (x input) with
-  | ParseError _ at -> ((List.Tot.rev prev_a),at)
+  | ParseError _ at -> 
+     substring_is_reflexive input;
+     ((List.Tot.rev prev_a),input)
   | Success v rest -> 
-     proper_substring_is_shorter rest input;
-     parse_star_aux rest x (v :: prev_a)
+     if rest = input then ((List.Tot.rev prev_a),input)
+       else ( substring_is_shorter rest input;
+              proper_substring rest input;
+              let next_match = parse_star_aux rest x (v :: prev_a) in
+                ( substring_transitivity (snd next_match) rest input;
+                  assert( is_substring (snd next_match) input );
+                  // OK, this is dumb, F* knows about (snd next_match) but it
+                  // can't apply that to intrinsic type of the pair without
+                  // me spelling it out for it.
+                  ((fst next_match), (snd next_match)) ) )
 
 // Parse zero or more of the given parser, returned as a list
-let parse_star #a (x:(proper_parser a)) : Tot (parser (list a)) =
+let parse_star #a (x:(parser a)) : Tot (parser (list a)) =
   fun (input:string) -> 
      let r = parse_star_aux input x [] in
        Success (fst r) (snd r)
+
+let listify #a (x:a) : y:(list a){Cons? y} = [x]
+
+// Parse one or more of the given parser, returned as a list
+let parse_plus #a (x:(parser a)) : Tot (parser (z:(list a){Cons? z})) =
+  parse_nonempty_list (parse_apply listify x) (parse_star x)
 
 (*
   Parsers for basic types
 *)
 
 // Return the string when the string is matched.
-let literal (a:string) (input:string) : Tot (parse_result string) =
+let literal (a:string) : Tot (parser (m:string{m=a})) = 
+  fun (input:string) ->
   if strlen a > strlen input then
      ParseError (sprintf "literal '%s'" a) input
   else let m = sub input 0 (strlen a) in
@@ -154,14 +178,19 @@ let literal (a:string) (input:string) : Tot (parse_result string) =
         ParseError (sprintf "literal '%s'" a) input
 
 // Return a specific value when the string is matched
-let literal_of #b (a:string) (v:b) (input:string) : Tot (parse_result b) =
+let literal_of #b (a:string) (v:b) (input:string) : Tot (parse_result (m:b{m==v})) =
   match literal a input with
   | ParseError expected at -> ParseError expected at
   | Success _ rest -> Success v rest
 
-(*
+type digit_string = (x:string{x = "0" || x = "1" || x = "2" || x = "3" || x = "4" || x = "5" || x = "6" || x = "7" || x = "8" || x = "9"})
+
+let digit : (parser digit_string) =
+    literal "0" <|> literal "1" <|> literal "2" <|> literal "3"
+  
+
 let integer (input:string) : Tot (parse_result int) = 
-  *)
+  
 
 
   
