parser/StringLemmas.fst
@@ -1,0 +1,123 @@
+module StringLemmas
+
+open FStar.String
+open FStar.List.Tot
+open FStar.Classical
+     
+// Need to define substrings to state that the parser consumes
+// a portion of the input and leaves the rest.
+let is_substring (a:string) (b:string) : bool = 
+  if strlen a = 0 then true else
+  if strlen a > strlen b then false else
+  (sub b 0 (strlen a)) = a
+
+// First n elmements of a list
+let rec first_n #a (n:nat) (l:(list a){length l >= n}) : (x:(list a){length x = n}) =
+  if n = 0 then []
+  else match l with
+  | hd :: tl -> hd :: (first_n (n-1) tl)
+
+// Sublist of a list starting at i and taking j elements
+let rec sublist #a (i:nat) (n:nat) (l:(list a){length l >= i+n}) : (x:(list a){length x = n}) =
+  if n = 0 then []
+  else if i > 0 then match l with
+  | hd :: tl -> (sublist (i-1) n tl)
+  else match l with
+  | hd :: tl -> hd :: (sublist 0 (n-1) tl)
+
+// Taking the entire sublist gives an equal string
+let rec sublist_of_whole_length #a (l:(list a)) : 
+  Lemma (ensures (sublist 0 (length l) l) == l )
+  = match l with 
+   | [] -> ()
+   | hd ::tl -> sublist_of_whole_length tl
+
+// Taking a sublist of a sublist gives the shorter sublist
+let rec sublist_of_sublist_is_sublist #a (l:(list a)) (x:nat{length l >= x}) (y:nat{y <= x}) 
+ : Lemma (ensures (sublist 0 y l) == (sublist 0 y (sublist 0 x l)))
+  = if y = 0 then ()
+    else match l with
+    hd :: tl -> sublist_of_sublist_is_sublist tl (x-1) (y-1)
+    
+// String lemmas: have to admit because no model exists, and 
+// standard library lemmas are not strong enough; they don't state anything
+// about sub.
+// This is my attempt to define sub in terms of things that *are* strong enough
+// to reason about.
+let substring_is_sublist (s:string) (i:nat) (l:nat{i+l <= strlen s}) : 
+  Lemma (ensures (sub s i l) =
+                 (string_of_list (sublist i l (list_of_string s))))
+     = admit()
+
+// Derived lemmas
+let all_strings_of_length_zero_are_equal (s:string{strlen s=0}) (t:string{strlen t=0}) 
+  : Lemma (ensures (s=t)) = 
+    // assert( list_of_string s = [] );
+    // assert( list_of_string t = [] );
+    string_of_list_of_string s;
+    string_of_list_of_string t
+
+let substring_of_length_is_equal (s:string)
+ : Lemma (ensures (sub s 0 (strlen s)) = s )
+   = substring_is_sublist s 0 (strlen s);
+     sublist_of_whole_length (list_of_string s);
+     // assert( sublist 0 (strlen s) (list_of_string s) = (list_of_string s) );
+     string_of_list_of_string s
+
+let substring_is_reflexive (s:string)
+ : Lemma (ensures is_substring s s)
+   = substring_of_length_is_equal s
+
+let substring_is_shorter (a:string) (b:string) 
+ : Lemma (requires (is_substring a b))
+         (ensures (strlen a) <= (strlen b) )
+   = ()
+
+let substring_of_substring_is_substring (s:string) (x:nat{strlen s >= x}) (y:nat{y <= x})
+ : Lemma (ensures (sub s 0 y) == (sub (sub s 0 x) 0 y))
+ = sublist_of_sublist_is_sublist (list_of_string s) x y;
+   //     (sublist 0 y (list_of_string s))
+   // ==  (sublist 0 y (sublist 0 x (list_of_string s)))
+   // therefore 
+   //     (s_o_l (sublist 0 y (list_of_string s)))
+   // ==  (s_o_l (sublist 0 y (sublist 0 x (list_of_string s))))
+   substring_is_sublist s 0 y;
+   // therefore
+   assert( (sub s 0 y) == string_of_list (sublist 0 y (sublist 0 x (list_of_string s))));
+   // To simplify the right hand side we need to inject a l_o_s/s_o_l pair
+   // in front of (sublist 0 x ...)
+   list_of_string_of_list (sublist 0 x (list_of_string s));
+   // Then simplify to (sub s 0 y) == (sub XXXXXXX o y)
+   substring_is_sublist (string_of_list (sublist 0 x (list_of_string s))) 0 y;
+   substring_is_sublist s 0 x
+   
+// Lemma: a substring of a substring is a substring
+let substring_transitivity (a:string) (b:string) (c:string) :
+  Lemma (requires (is_substring a b) /\ (is_substring b c))
+        (ensures (is_substring a c)) 
+       // (sub c 0 (strlen b)) = b
+       // (sub b 0 (strlen a)) = a     
+       // WTP: (sub c 0 (strlen a)) = a
+     = substring_is_shorter a b;  // (strlen a) <= (strlen b)
+       substring_of_substring_is_substring c (strlen b) (strlen a)
+       
+// Lemma if a and b are the same length, then if a is a substring of b,
+// they must be equal.
+let substring_equality (a:string) (b:string) :
+  Lemma (requires (is_substring a b) /\ (strlen a) = (strlen b))
+        (ensures (a=b))
+   = if strlen a = 0 then
+     all_strings_of_length_zero_are_equal a b
+   else
+     assert (sub b 0 (strlen a) = a);
+     substring_of_length_is_equal b
+
+// Lemma: if x is a substring of y, and x != y, then strlen x < strlen y
+let proper_substring (a:string) (b:string)
+: Lemma ( requires (is_substring a b) /\ (a <> b) )
+  ( ensures (strlen a) < (strlen b)) = 
+  substring_is_shorter a b;
+  // Convert substring_equality into an implication, so we can apply modus tollens
+  move_requires_2 substring_equality a b
+
+
