parser/StringLemmas.fsti
@@ -1,0 +1,43 @@
+module StringLemmas
+
+open FStar.String
+
+val is_substring (a:string) (b:string) : bool
+
+// If two strings have zero length, they are equal.
+val all_strings_of_length_zero_are_equal (s:string{strlen s=0}) (t:string{strlen t=0}) 
+ : Lemma (ensures (s=t))
+
+// A substring of the same length as the original, is the original
+val substring_of_length_is_equal (s:string) 
+ : Lemma (ensures (sub s 0 (strlen s)) = s )
+
+// All strings are substrings of themeselves
+val substring_is_reflexive (s:string)
+ : Lemma (ensures is_substring s s)
+
+// The substring relationship imposes an order on string length
+val substring_is_shorter (a:string) (b:string) 
+ : Lemma (requires (is_substring a b))
+         (ensures (strlen a) <= (strlen b) )
+
+// Taking a shorter substring of a longer substring gives the shorter substring
+val substring_of_substring_is_substring (s:string) (x:nat{strlen s >= x}) (y:nat{y <= x})
+ : Lemma (ensures (sub s 0 y) == (sub (sub s 0 x) 0 y))
+
+// is_substring is a transitive relationship
+val substring_transitivity (a:string) (b:string) (c:string)
+ : Lemma (requires (is_substring a b) /\ (is_substring b c))
+         (ensures (is_substring a c)) 
+
+// If a and b are the same length, and a is a substring of b,
+// they must be equal.
+val substring_equality (a:string) (b:string) :
+  Lemma (requires (is_substring a b) /\ (strlen a) = (strlen b))
+        (ensures (a=b))
+
+// If x is a substring of y, and x != y, then strlen x < strlen y
+val proper_substring (a:string) (b:string)
+ : Lemma (requires (is_substring a b) /\ (a <> b))
+         (ensures (strlen a) < (strlen b))
+         
